Fix the misused max''

Examples/min_idx2.v
@@ -1,7 +1,7 @@
 Require Import Monad SkelLib Computation ZArith TypedTerm Program.
 Open Scope Z_scope.
 
-Definition max_idx (arr : list Z) : comp (list (Z * Z))
+Definition min_idx (arr : list Z) : comp (list (Z * Z))
   :=
   reduceM (fun x y => if (fst x) <? (fst y)
                       then ret x else ret y)
@@ -12,10 +12,10 @@ Lemma zip_seq (arr : list Z) :
   gen (fun i => do! x := nth_error arr i in ret (x, i)) (len arr).
 Admitted.
 
-Definition max_idx_IR:  {p : Skel.AS (Skel.TZ :: nil) (Skel.TTup Skel.TZ Skel.TZ) |
-      equiv1 p (max_idx)}.
+Definition min_idx_IR:  {p : Skel.AS (Skel.TZ :: nil) (Skel.TTup Skel.TZ Skel.TZ) |
+      equiv1 p (min_idx)}.
 Proof.
-  unfold max_idx.
+  unfold min_idx.
 
   simpl in *.
   eapply change_spec; [intros; eapply ext_fun; [intros|]|].
@@ -65,13 +65,13 @@ Defined.
 
 Require Import Compiler Ext Extract.
 
-Definition max_idx_CUDA : Host.Prog :=
-  match max_idx_IR with
+Definition min_idx_CUDA : Host.Prog :=
+  match min_idx_IR with
   | exist ir _ =>
     Compiler.compile_prog 1024 24 ir
   end.
 
-Definition res := save_to_file max_idx_CUDA "max_idx_opt.cu".
+Definition res := save_to_file min_idx_CUDA "min_idx_opt.cu".
 
 Cd "extracted".
 
